theories/interop/wp_ext_call_laws.v
@@ -1,8 +1,8 @@
 From melocoton.mlanguage Require Import weakestpre.
 From melocoton.interop.wp_prims Require Export
-  alloc alloc_foreign int2val isblock length modify readfield
+  (* alloc alloc_foreign *) int2val isblock length (* modify *) readfield
   read_foreign read_tag registerroot unregisterroot val2int
-  write_foreign.
+  (* write_foreign *).
 
 Section Laws.
 
@@ -19,19 +19,19 @@ Lemma base_prim_correct (p : prim) e Ψ :
 Proof using.
   intros Hncb Hnmain.
   (destruct p; try by congruence); unfold prim_proto.
-  - apply alloc_correct.
+  - admit; apply alloc_correct.
   - apply registerroot_correct.
   - apply unregisterroot_correct.
-  - apply modify_correct.
+  - admit; apply modify_correct.
   - apply readfield_correct.
   - apply val2int_correct.
   - apply int2val_correct.
   - apply isblock_correct.
   - apply read_tag_correct.
   - apply length_correct.
-  - apply alloc_foreign_correct.
-  - apply write_foreign_correct.
+  - admit; apply alloc_foreign_correct.
+  - admit; apply write_foreign_correct.
   - apply read_foreign_correct.
-Qed.
+Admitted.
 
 End Laws.
